src/derivable_tools.v
@@ -1,15 +1,258 @@
 From mathcomp Require Import ssreflect ssrbool ssrfun.
-From mathcomp Require Import eqtype seq order.
+From mathcomp Require Import ssrnat eqtype seq order.
 From ipcssr Require Import prelude forms derivations derivable_def.
 
 Section Derivable.
 Context {A : Type}.
 
 Lemma derivable_weak ctx (a b : form A) :
- Derivable ctx a -> Derivable (b :: ctx) a.
+  Derivable ctx a -> Derivable (b :: ctx) a.
 Proof.
 case=>t Dt; apply: (Derivable_Intro _ _ (Shift t)).
 by apply: ShiftIntro.
+Qed.
+
+Lemma derivable_weak_list ctx1 ctx2 (a : form A) :
+  Derivable ctx1 a -> Derivable (ctx2 ++ ctx1) a.
+Proof. by elim: ctx2=>//= b ctx2 /[apply]; apply: derivable_weak. Qed.
+
+Lemma derivable_cut_aux ctx t (b : form A) :
+  derives ctx t b ->
+  forall a l1 l2,
+  ctx = l1 ++ a :: l2 -> Derivable [::] a -> Derivable (l1 ++ l2) b.
+Proof.
+elim/(@derives_rec A)=>{ctx t b}.
+- move=>g n a + b l1 l2 E; rewrite {g}E onth_cat /=.
+  case: (ltngtP n (size l1))=>Hn.
+  - move=>H _; apply/(Derivable_Intro _ _ (Var n))/ByAssumption.
+    by rewrite onth_cat Hn.
+  - move=>Ha Db; apply/(Derivable_Intro _ _ (Var n.-1))/ByAssumption.
+    rewrite onth_cat ltnNge.
+    move: (Hn); rewrite -{1}(ltn_predK Hn) ltnS=>->/=.
+    rewrite -predn_sub; case Ek: (n - size l1) Ha=>[|k] //.
+    by move: Hn; rewrite -subn_gt0 Ek.
+  rewrite Hn subnn; case=>{b}-> D.
+  by rewrite -(cats0 (l1++l2)); apply: derivable_weak_list.
+- move=>g _ a _ IH b l1 l2 /IH/[apply]; case=>t Df.
+  by apply/(Derivable_Intro _ _ (Efq t a))/ByAbsurdity.
+- move=>g a _ b _ IH c l1 l2 E Dc.
+  case: (IH c (a::l1) l2)=>//= [|t Db]; first by rewrite E.
+  by apply/(Derivable_Intro _ _ (Abs a t))/ImpIntro.
+- move=>g _ _ a b _ IHab _ IHa c l1 l2 E Dc.
+  case: (IHab _ _ _ E Dc)=>r Dab.
+  case: (IHa _ _ _ E Dc)=>s Da.
+  by apply/(Derivable_Intro _ _ (App a r s))/ImpElim.
+- move=>g _ _ a b _ IHa _ IHb c l1 l2 E Dc.
+  case: (IHa _ _ _ E Dc)=>r Da.
+  case: (IHb _ _ _ E Dc)=>s Db.
+  by apply/(Derivable_Intro _ _ (Pair r s))/AndFIntro.
+- move=>g _ a b _ IH c l1 l2 E Dc.
+  case: (IH _ _ _ E Dc)=>t Dab.
+  by apply/(Derivable_Intro _ _ (PrL b t))/AndFElimL.
+- move=>g _ a b _ IH c l1 l2 E Dc.
+  case: (IH _ _ _ E Dc)=>t Dab.
+  by apply/(Derivable_Intro _ _ (PrR a t))/AndFElimR.
+- move=>g _ a b _ IH c l1 l2 E Dc.
+  case: (IH _ _ _ E Dc)=>t Da.
+  by apply/(Derivable_Intro _ _ (OrFL t b))/OrFIntroL.
+- move=>g _ a b _ IH c l1 l2 E Dc.
+  case: (IH _ _ _ E Dc)=>t Da.
+  by apply/(Derivable_Intro _ _ (OrFR t a))/OrFIntroR.
+- move=>g _ _ _ a b c _ IHab _ IHa _ IHb  d l1 l2 E Dd.
+  case: (IHab _ _ _ E Dd)=>r Dab.
+  case: (IHa d (a::l1) l2)=>//= [|s Da]; first by rewrite E.
+  case: (IHb d (b::l1) l2)=>//= [|t Db]; first by rewrite E.
+  by apply/(Derivable_Intro _ _ (Cas a b r s t))/OrFElim.
+move=>g r a b Dr IH c l1 l2 E Dc.
+case: l1 E=>/= [|a' l1]; case.
+- by move=>_ <-; apply/Derivable_Intro/Dr.
+move=><- E; case: (IH _ _ _ E Dc)=>t Dt.
+by apply/derivable_weak/Derivable_Intro/Dt.
+Qed.
+
+Lemma derivable_cut ctx (a b : form A) :
+  Derivable [::] a -> Derivable (a :: ctx) b -> Derivable ctx b.
+Proof.
+move=>Da; case=>t Db; rewrite -(cat0s ctx).
+by apply/(derivable_cut_aux _ _ _ Db)/Da.
+Qed.
+
+Lemma derivable_cut_merge ctx (a b : form A) :
+  Derivable ctx a -> Derivable (a :: ctx) b -> Derivable ctx b.
+Proof.
+elim: ctx=>[|c ctx IH] in a b *.
+- by apply: derivable_cut.
+move=>Da Db.
+case: (IH (Imp c a) (Imp c b)).
+- by case: Da=>t Dt; apply/(Derivable_Intro _ _ (Abs c t))/ImpIntro.
+- case: Db=>t Dt.
+  apply: (Derivable_Intro _ _ (Abs c (App a (App c (Shift (Shift (Abs c (Abs a t)))) (Var 0))
+                                            (App c (Var 1) (Var 0))))).
+  apply/ImpIntro/ImpElim.
+  - apply/ImpElim; last by apply: ByAssumption.
+    by apply/ShiftIntro/ShiftIntro/ImpIntro/ImpIntro.
+  by apply/ImpElim; apply: ByAssumption.
+move=>t Dt; apply (Derivable_Intro _ _(App c (Shift t) (Var 0))).
+apply/ImpElim; last by apply: ByAssumption.
+by apply/ShiftIntro.
+Qed.
+
+(************************************************************************)
+
+Lemma derivable_a_imp_a (a : form A) : Derivable [::] (Imp a a).
+Proof.
+by apply/(Derivable_Intro _ _ (Abs a (Var 0)))/ImpIntro/ByAssumption.
+Qed.
+
+Lemma derivable_a_and_b__derivable_a ctx (a b : form A) :
+  Derivable ctx (AndF a b) -> Derivable ctx a.
+Proof. by case=>t Dt; apply/(Derivable_Intro _ _ (PrL b t))/AndFElimL. Qed.
+
+Lemma derivable_a_and_b__derivable_b ctx (a b : form A) :
+  Derivable ctx (AndF a b) -> Derivable ctx b.
+Proof. by case=>t Dt; apply/(Derivable_Intro _ _ (PrR a t))/AndFElimR. Qed.
+
+Lemma derivable_falsum_or_a__derivable_a ctx (a : form A) :
+  Derivable ctx (OrF Falsum a) -> Derivable ctx a.
+Proof.
+case=>t Dt.
+apply/(Derivable_Intro _ _ (Cas Falsum a t (Efq (Var 0) a) (Var 0)))/OrFElim=>//.
+- by apply/ByAbsurdity/ByAssumption.
+by apply/ByAssumption.
+Qed.
+
+Lemma derivable_a_or_falsum__derivable_a ctx (a : form A) :
+  Derivable ctx (OrF a Falsum) -> Derivable ctx a.
+Proof.
+case=>t Dt.
+apply/(Derivable_Intro _ _ (Cas a Falsum t (Var 0) (Efq (Var 0) a)))/OrFElim=>//.
+- by apply/ByAssumption.
+by apply/ByAbsurdity/ByAssumption.
+Qed.
+
+Lemma derivable_a_imp_falsum_or_b__derivable_a_imp_b ctx (a b : form A) :
+  Derivable ctx (Imp a (OrF Falsum b)) -> Derivable ctx (Imp a b).
+Proof.
+case=>t Dt.
+apply/(Derivable_Intro _ _ (Abs a (Cas Falsum b (App a (Shift t) (Var 0)) (Efq (Var 0) b) (Var 0))))/ImpIntro/OrFElim.
+- by apply: ImpElim; [apply: ShiftIntro | apply: ByAssumption].
+- by apply/ByAbsurdity/ByAssumption.
+by apply: ByAssumption.
+Qed.
+
+Lemma derivable_a_imp_b_or_falsum__derivable_a_imp_b ctx (a b : form A) :
+  Derivable ctx (Imp a (OrF b Falsum)) -> Derivable ctx (Imp a b).
+Proof.
+case=>t Dt.
+apply/(Derivable_Intro _ _ (Abs a (Cas b Falsum (App a (Shift t) (Var 0)) (Var 0) (Efq (Var 0) b))))/ImpIntro/OrFElim.
+- by apply: ImpElim; [apply: ShiftIntro | apply: ByAssumption].
+- by apply: ByAssumption.
+by apply/ByAbsurdity/ByAssumption.
+Qed.
+
+Lemma derivable_a_and_b_imp_c__derivable_a_imp_b_imp_c ctx (a b c : form A) :
+  Derivable ctx (Imp (AndF a b) c) -> Derivable ctx (Imp a (Imp b c)).
+Proof.
+case=>t Dt.
+apply: (Derivable_Intro _ _ (Abs a (Abs b (App (AndF a b) (Shift (Shift t)) (Pair (Var 1) (Var 0)))))).
+apply/ImpIntro/ImpIntro/ImpElim.
+- by apply/ShiftIntro/ShiftIntro.
+by apply: AndFIntro; apply: ByAssumption.
+Qed.
+
+Lemma derivable_a_or_b_imp_c__derivable_a_imp_b ctx (a b c : form A) :
+  Derivable ctx (Imp (OrF a b) c) -> Derivable ctx (Imp a c).
+Proof.
+case=>t Dt.
+apply: (Derivable_Intro _ _ (Abs a (App (OrF a b) (Shift t) (OrFL (Var 0) b)))).
+apply/ImpIntro/ImpElim.
+- by apply: ShiftIntro.
+by apply/OrFIntroL/ByAssumption.
+Qed.
+
+Lemma derivable_a_or_b_imp_c__derivable_b_imp_c ctx (a b c : form A) :
+  Derivable ctx (Imp (OrF a b) c) -> Derivable ctx (Imp b c).
+Proof.
+case=>t Dt.
+apply: (Derivable_Intro _ _(Abs b (App (OrF a b) (Shift t) (OrFR (Var 0) a)))).
+apply/ImpIntro/ImpElim.
+- by apply: ShiftIntro.
+by apply/OrFIntroR/ByAssumption.
+Qed.
+
+Lemma derivable_falsum_imp_b_imp_c__derivable_c ctx (b c : form A) :
+  Derivable ctx (Imp (Imp Falsum b) c) -> Derivable ctx c.
+Proof.
+case=>t Dt.
+apply: (Derivable_Intro _ _ (App (Imp Falsum b) t (Abs Falsum (Efq (Var 0) b)))).
+apply: ImpElim=>//.
+by apply/ImpIntro/ByAbsurdity/ByAssumption.
+Qed.
+
+Lemma derivable_b__derivable_a_imp_b ctx (a b : form A) :
+  Derivable ctx b -> Derivable ctx (Imp a b).
+Proof.
+case=>t Dt.
+by apply/(Derivable_Intro _ _ (Abs a (Shift t)))/ImpIntro/ShiftIntro.
+Qed.
+
+Lemma derivable_a_a_imp_b__derivable_b ctx (a b : form A) :
+  Derivable ctx a -> Derivable ctx (Imp a b) -> Derivable ctx b.
+Proof.
+case=>t Dt; case=>s Ds.
+by apply/(Derivable_Intro _ _  (App a s t))/ImpElim.
+Qed.
+
+Lemma derivable_a_context_b__derivable_a_imp_b ctx (a b : form A) :
+  Derivable (a :: ctx) b -> Derivable ctx (Imp a b).
+Proof.
+case=>t Dt.
+by apply/(Derivable_Intro _ _ (Abs a t))/ImpIntro.
+Qed.
+
+Lemma derivable_vimp ctx l (a b : form A) :
+  (forall ctx, Derivable ctx a -> Derivable ctx b) ->
+  Derivable ctx (vimp l a) -> Derivable ctx (vimp l b).
+Proof.
+elim: l=>[|c l IH] /= in a b *; move=>H.
+- by apply: H.
+apply: IH=>{}ctx.
+case=>t Dt; case: (H (Atom c::ctx)).
+- apply: (Derivable_Intro _ _ (App (Atom c) (Shift t) (Var 0))).
+  by apply/ImpElim; [apply: ShiftIntro | apply: ByAssumption].
+move=>s Ds; apply: (Derivable_Intro _ _ (Abs (Atom c) s)).
+by apply: ImpIntro.
+Qed.
+
+Lemma derivable_vimp2 ctx l (a b c : form A) :
+  (forall ctx,
+   Derivable ctx a -> Derivable ctx b -> Derivable ctx c) ->
+  Derivable ctx (vimp l a) -> Derivable ctx (vimp l b) ->
+  Derivable ctx (vimp l c).
+Proof.
+elim: l=>[|d l IH] /= in a b c *; move=> H.
+- by apply: H.
+apply: IH=>{}ctx.
+case=>t Dt; case=>s Ds.
+case: (H (Atom d::ctx)).
+- apply: (Derivable_Intro _ _ (App (Atom d) (Shift t) (Var 0))).
+  by apply/ImpElim; [apply: ShiftIntro | apply: ByAssumption].
+- apply: (Derivable_Intro _ _ (App (Atom d) (Shift s) (Var 0))).
+  by apply/ImpElim; [apply: ShiftIntro | apply: ByAssumption].
+move=>q Dq; apply: (Derivable_Intro _ _ (Abs (Atom d) q)).
+by apply: ImpIntro.
+Qed.
+
+Lemma derivable_vimp0 ctx l (a : form A) :
+  (forall ctx, Derivable ctx a) ->
+  Derivable ctx (vimp l a).
+Proof.
+elim: l=>[|b l IH] /= in a *; move=>H.
+- by apply: H.
+apply: IH=>{}ctx.
+case: (H (Atom b::ctx))=>t Dt.
+apply: (Derivable_Intro _ _ (Abs (Atom b) t)).
+by apply: ImpIntro.
 Qed.
 
 End Derivable.
@@ -73,12 +316,3 @@ by apply: derivable_subst.
 Qed.
 
 End DerivableOrd.
-
-
-(*
-From Coq Require Extraction ExtrOcamlBasic ExtrOcamlNatInt.
-
-Extract Inductive reflect => bool [ true false ].
-
-Extraction "ext.ml" derivable_subst.
-*)
