src/nminimal.v
@@ -1,0 +1,166 @@
+From mathcomp Require Import ssreflect ssrbool ssrfun.
+From mathcomp Require Import ssrnat seq eqtype order.
+From ipcssr Require Import prelude avlmap forms derivations normal_forms kripke_trees in_ngamma forces_ngamma le_ks derivable_def.
+
+Section NMinimal.
+Context {disp : unit} {A : orderType disp}.
+
+Definition nminimal (work : seq (normal_form A)) (ds : seq (disj A)) (ni : seq (nested_imp A))
+                    (ai : atomic_imps A) (a : atoms A) (ctx : seq (form A)) :=
+  forall k, Is_Monotone_kripke_tree k ->
+    forces_ngamma work ds ni ai a k -> {in ctx, forall c, forces_t k c}.
+
+(*********************************************************************)
+
+Lemma nminimal_derivable_forces work ds ni ai a ctx k :
+  Is_Monotone_kripke_tree k ->
+  forces_ngamma work ds ni ai a k ->
+  nminimal work ds ni ai a ctx ->
+  forall c, Derivable ctx c -> forces_t k c.
+Proof.
+move=>M F N c; case=>t D.
+by apply/(soundness_t _ _ _ D _ M)/N.
+Qed.
+
+(*********************************************************************)
+
+Lemma nminimal_eqv work ds ni1 ni2 ai a ctx :
+  eqv_ni ni1 ni2 ->
+  nminimal work ds ni1 ai a ctx -> nminimal work ds ni2 ai a ctx.
+Proof.
+rewrite /nminimal=>E NM k M F.
+by apply: NM=>//; apply/forces_ngamma_eqv/F.
+Qed.
+
+(************************************************************************)
+
+Lemma nminimal_shift_work_ds i j work ds ni ai a ctx :
+  nminimal (NDisj i j :: work) ds ni ai a ctx ->
+  nminimal work ((i, j) :: ds) ni ai a ctx.
+Proof.
+rewrite /nminimal=>NM k M F.
+by apply: NM=>//; apply: forces_ngamma_shift_ds_work.
+Qed.
+
+Lemma nminimal_shift_work_ni x work ds ni ai a ctx :
+  nminimal (NImp_NF (nested_imp2nimp x) :: work) ds ni ai a ctx ->
+  nminimal work ds (x :: ni) ai a ctx.
+Proof.
+rewrite /nminimal=>NM k M F.
+by apply: NM=>//; apply: forces_ngamma_shift_ni_work.
+Qed.
+
+Lemma nminimal_shift_work_ai i b work ds ni ai a ctx :
+  invariant ai ->
+  nminimal (AImp i b :: work) ds ni ai a ctx ->
+  nminimal work ds ni (update_aimps b i ai) a ctx.
+Proof.
+rewrite /nminimal=>Ha NM k M F.
+by apply: NM=>//; apply: forces_ngamma_shift_ai_work.
+Qed.
+
+(*
+Lemma nminimal_shift_work_ai_new i b work ds ni ai a ctx :
+  invariant ai -> ~~ lookup ai i ->
+  nminimal (AImp i b :: work) ds ni ai a ctx ->
+  nminimal work ds ni (update_aimps b i ai) a ctx.
+Proof.
+rewrite /nminimal=>Ha L NM k M F.
+by apply: NM=>//; apply: forces_ngamma_shift_ai_work_new.
+Qed.
+
+Lemma nminimal_shift_work_ai_old i b work ds ni ai a ctx :
+  invariant ai -> lookup ai i ->
+  nminimal (AImp i b :: work) ds ni ai a ctx ->
+  nminimal work ds ni (update_aimps b i ai) a ctx.
+Proof.
+rewrite /nminimal=>Ha L NM k M F.
+by apply: NM=>//; apply: forces_ngamma_shift_ai_work_old.
+Qed.
+*)
+
+Lemma nminimal_shift_work_a i work ds ni ai a ctx :
+  invariant a ->
+  nminimal (NAtom i :: work) ds ni ai a ctx ->
+  nminimal work ds ni ai (update_atoms i a) ctx.
+Proof.
+rewrite /nminimal=>Ha NM k M F.
+by apply: NM=>//; apply: forces_ngamma_shift_a_work.
+Qed.
+
+Lemma nminimal_shift_work_ni_x_ni x work ds ni1 ni2 ai a ctx :
+  nminimal (NImp_NF (nested_imp2nimp x) :: work) ds (ni1 ++ ni2) ai a ctx ->
+  nminimal work ds (ni1 ++ x :: ni2) ai a ctx.
+Proof.
+rewrite /nminimal=>NM k M F.
+by apply: NM=>//; apply: forces_ngamma_shift_ni_x_ni_work.
+Qed.
+
+Lemma nminimal_shift_ni_x_ni_work x work ds ni1 ni2 ai a ctx :
+  nminimal work ds (ni1 ++ x :: ni2) ai a ctx ->
+  nminimal (NImp_NF (nested_imp2nimp x) :: work) ds (ni1 ++ ni2) ai a ctx.
+Proof.
+rewrite /nminimal=>NM k M F.
+by apply: NM=>//; apply: forces_ngamma_shift_work_ni_x_ni.
+Qed.
+
+(********************************************************************)
+
+Lemma nminimal_cons_work_strength b c work ds ni ai a ctx :
+  (forall k, Is_Monotone_kripke_tree k ->
+   forces_ngamma (c :: work) ds ni ai a k -> forces_t k (nf2form b)) ->
+  nminimal (b :: work) ds ni ai a ctx ->
+  nminimal (c :: work) ds ni ai a ctx.
+Proof.
+rewrite /nminimal=>H NM k M F.
+apply: NM=>//; apply: (forces_ngamma_cons_work_weak c)=>// F'.
+by apply: H.
+Qed.
+
+Lemma nminimal_cons_work_weak b c work ds ni ai a ctx :
+  (forall k, Is_Monotone_kripke_tree k ->
+   forces_t k (nf2form c) -> forces_t k (nf2form b)) ->
+  nminimal (b :: work) ds ni ai a ctx ->
+  nminimal (c :: work) ds ni ai a ctx.
+Proof.
+rewrite /nminimal=>H NM k M F.
+apply: NM=>//; apply: (forces_ngamma_cons_work_weak c)=>// F'.
+by apply: H.
+Qed.
+
+Lemma nminimal_shift_work_ai_weak i bs work ds ni ai a ctx :
+  invariant ai -> lookup ai i = Some bs ->
+  nminimal work ds ni ai a ctx ->
+  nminimal (bs ++ work) ds ni (delete i ai) a ctx.
+Proof.
+rewrite /nminimal=>Ha L NM k M F.
+apply: NM=>//; apply: (forces_ngamma_del_ai_rev i bs)=>//.
+- move=>n b E; rewrite /nf2form -/nf2form.
+  apply: forces_imp_t=>//; apply/F/(In_Work _ _ _ _ _ n).
+  by rewrite onth_cat (onth_size E).
+by apply: (forces_ngamma_cat_work_tail bs).
+Qed.
+
+Lemma nminimal_shift_ds_work_context work c i j ds ni ai a ctx :
+  (forall k, Is_Monotone_kripke_tree k ->
+   forces_t k (nf2form c) -> forces_t k (OrF (Atom i) (Atom j))) ->
+  nminimal work ((i, j) :: ds) ni ai a ctx ->
+  nminimal (c :: work) ds ni ai a (nf2form c :: ctx).
+Proof.
+rewrite /nminimal=>H NM k M F d; rewrite inE; case/orP=>[/eqP{d}->|Hd].
+- by apply/F/in_ngamma_cons_work_head.
+apply: NM=>//; apply/forces_ngamma_shift_work_ds.
+apply/(forces_ngamma_cons_work_weak c)=>// Fc.
+by rewrite /nf2form -/nf2form; apply: H.
+Qed.
+
+Lemma nminimal_cons_work_cons_context c work ds ni ai a ctx :
+  nminimal work ds ni ai a ctx ->
+  nminimal (c :: work) ds ni ai a (nf2form c :: ctx).
+Proof.
+rewrite /nminimal=>NM k M F d; rewrite inE; case/orP=>[/eqP{d}->|Hd].
+- by apply/F/in_ngamma_cons_work_head.
+by apply: NM=>//; apply/(forces_ngamma_cons_work_tail c).
+Qed.
+
+End NMinimal.
